Add boilerplate to State* files to get decls to go through for several XMM instructions.  Interestingly, poly now needs extra rlimit to go through

src/arch/x64/X64.Vale.StateLemmas_i.fst
@@ -10,14 +10,16 @@ module M = TransparentMap
 let state_to_S (s:state) : S.state = {
   S.ok = s.ok;
   S.regs = (fun r -> s.regs r);
+  S.xmms = (fun x -> s.xmms x);
   S.flags = int_to_nat64 s.flags;
   S.mem = s.mem;
 }
 
 let state_of_S (s:S.state) : state =
-  let { S.ok = ok; S.regs = regs; S.flags = flags; S.mem = mem } = s in {
+  let { S.ok = ok; S.regs = regs; S.xmms = xmms; S.flags = flags; S.mem = mem } = s in {
     ok = ok;
     regs = (fun r -> regs r);
+    xmms = (fun x -> xmms x);
     flags = flags;
     mem = mem;
   }
@@ -26,7 +28,9 @@ let lemma_to_ok s = ()
 let lemma_to_flags s = ()
 let lemma_to_mem s = ()
 let lemma_to_reg s r = ()
+let lemma_to_xmm s x = ()
 let lemma_to_eval_operand s o = ()
+let lemma_to_eval_xmm s x = ()
 let lemma_to_valid_operand s o = ()
 
 let lemma_of_to s =
@@ -36,7 +40,8 @@ let lemma_of_to s =
 let lemma_to_of s =
   let s' = state_of_S s in
   let s'' = state_to_S s' in
-  let { S.ok = ok; S.regs = regs; S.flags = flags; S.mem = mem } = s in
-  let { S.ok = ok''; S.regs = regs''; S.flags = flags''; S.mem = mem'' } = s'' in
+  let { S.ok = ok; S.regs = regs; S.xmms = xmms; S.flags = flags; S.mem = mem } = s in
+  let { S.ok = ok''; S.regs = regs''; S.xmms = xmms''; S.flags = flags''; S.mem = mem'' } = s'' in
   assert (feq regs regs'');
+  assert (feq xmms xmms'');
   ()
