src/arch/x64/X64.Vale.StateLemmas_i.fsti
@@ -8,6 +8,7 @@ module M = TransparentMap
 
 unfold let ok' = S.Mkstate?.ok
 unfold let regs' = S.Mkstate?.regs
+unfold let xmms' = S.Mkstate?.xmms
 unfold let flags' = S.Mkstate?.flags
 unfold let mem' = S.Mkstate?.mem
 
@@ -30,9 +31,17 @@ val lemma_to_reg : s:state -> r:reg -> Lemma
   (ensures s.regs r == regs' (state_to_S s) r)
   [SMTPat (s.regs r)]
 
+val lemma_to_xmm : s:state -> x:xmm -> Lemma
+  (ensures s.xmms x == xmms' (state_to_S s) x)
+  [SMTPat (s.xmms x)]
+
 val lemma_to_eval_operand : s:state -> o:operand -> Lemma
   (ensures eval_operand o s == S.eval_operand o (state_to_S s))
   [SMTPat (eval_operand o s)]
+
+val lemma_to_eval_xmm : s:state -> x:xmm -> Lemma
+  (ensures eval_xmm x s == S.eval_xmm x (state_to_S s))
+  [SMTPat (eval_xmm x s)]
 
 val lemma_to_valid_operand : s:state -> o:operand -> Lemma
   (ensures valid_operand o s ==> S.valid_operand o (state_to_S s))
